concur/CallConvAlgebra.v
@@ -1,0 +1,132 @@
+Require Export LogicalRelations.
+Require Export List.
+Require Export Globalenvs.
+Require Export Events.
+Require Export LanguageInterface.
+
+Require Import Axioms.
+Require Import Coqlib.
+Require Import Integers.
+Require Import Values.
+Require Import Memory.
+
+Require Export CallconvBig.
+
+(** Algebraic structures on calling conventions. *)
+
+(** * Refinement and equivalence *)
+
+(** ** Definition *)
+
+(** The following relation asserts that the calling convention [cc] is
+  refined by the calling convention [cc'], meaning that any
+  [cc']-simulation is also a [cc]-simulation. *)
+
+(** cc1: internal, i.e. injp ⋅ injp
+    cc2: external, i.e. injp  *)
+
+
+(** We are trying to define the ccref_outgoing with respect to the "living wp1, however,
+    to show from [wp1 *-> (get w1)] we can construct w2 and show [wp2 *-> (get w2)], we still
+    have to show that wp1 and wp2 are recording the same injected memories. Such relation has to be **defined**
+    in some way "*)
+
+Import GS. 
+Definition ccref_outgoing {li1 li2} (cc1 cc2: callconv li1 li2) (match12 : gworld cc1 -> gworld cc2 -> Prop) :=
+  forall wp1 wp2 w1 se1 se2 q1 q2,
+    match_senv cc1 w1 se1 se2 ->
+    match_query cc1 w1 q1 q2 ->
+    wp1 *-> (get w1) ->
+    match12 wp1 wp2 ->
+    exists w2,
+      wp2 *-> (get w2) /\
+      match_senv cc2 w2 se1 se2 /\
+      match_query cc2 w2 q1 q2 /\
+      forall r1 r2 (wp2': gworld cc2),
+        get w2 o-> wp2' ->
+        match_reply cc2 (set w2 wp2') r1 r2 ->
+        exists (wp1' : gworld cc1),
+        get w1 o-> wp1' /\
+        match_reply cc1 (set w1 wp1') r1 r2 /\
+        match12 wp1' wp2'.            
+
+Definition ccref_incoming {li1 li2} (cc1 cc2: callconv li1 li2) (match12 : gworld cc1 -> gworld cc2 -> Prop):=
+  forall w2 se1 se2 q1 q2,
+    match_senv cc2 w2 se1 se2 ->
+    match_query cc2 w2 q1 q2 ->
+    exists (w1: ccworld cc1) ,
+      match_senv cc1 w1 se1 se2 /\
+      match_query cc1 w1 q1 q2 /\
+      match12 (get w1) (get w2) /\
+        (forall r1 r2 wp1 wp2 wp1',
+        match12 wp1 wp2 ->    
+        get w1 o-> wp1' -> wp1 *-> wp1' ->
+        match_reply cc1 (set w1 wp1') r1 r2 ->
+        exists (wp2' : gworld cc2),
+        (* match12 wp1' wp2' ->*)
+        get w2 o-> wp2' /\ wp2 *-> wp2' /\
+        match_reply cc2 (set w2 wp2') r1 r2).
+
+
+Record cctrans {li1 li2} (cc1 cc2: callconv li1 li2) :=
+  Callconv_Trans{
+        match12 : gworld cc1 -> gworld cc2 -> Prop;
+        big_step_incoming : ccref_incoming cc1 cc2 match12;
+        big_step_outgoing : ccref_outgoing cc1 cc2 match12;
+      }.
+
+  
+  Lemma open_fsim_cctrans {li1 li2: language_interface}:
+  forall (cc1 cc2: callconv li1 li2) L1 L2,
+    forward_simulation cc1 L1 L2 ->
+    cctrans cc1 cc2 ->
+    forward_simulation cc2 L1 L2.
+  (*cc1 : injp @ injp cc2: injp*)
+Proof.
+  intros.
+  destruct X as [match12 INCOM OUTGO].
+  inv H.
+  destruct X as [index order match_states SKEL PROP WF].
+  constructor.
+    set (ms se1 se2 (w2 : ccworld cc2) (wp2: gworld cc2) idx s1 s2 :=
+         exists w1 (wp1 : gworld cc1),
+           match_states se1 se2 w1 wp1 idx s1 s2 /\
+             match_senv cc1 w1 se1 se2 /\
+             match12 (get w1) (get w2) /\
+             match12 wp1 wp2 /\
+             (forall r1 r2 wp1 wp2 wp1', match12 wp1 wp2 -> (get w1) o-> wp1' -> wp1 *-> wp1' -> match_reply cc1 (set w1 wp1') r1 r2 ->
+            exists (wp2' : gworld cc2), (get w2) o-> wp2' /\ wp2 *-> wp2' /\ match_reply cc2 (set w2 wp2') r1 r2)).
+  eapply Forward_simulation with order ms; auto.
+  intros se1 se2 wB' Hse' Hse1.
+  split.
+  - intros q1 q2 Hq'.
+    destruct (INCOM wB' se1 se2 q1 q2) as (wB & Hse & Hq & Hr); auto.
+    eapply fsim_match_valid_query; eauto.
+  - intros q1 q2 s1 Hq' Hs1 Ho.
+    destruct (INCOM wB' se1 se2 q1 q2) as (wB & Hse & Hq & Htrans & Hf); auto.
+    edestruct @fsim_match_initial_states as (i & s2 & Hs2 & Hs); eauto.
+    exists i, s2. split; auto. red. exists wB,(get wB). repeat apply conj; eauto.
+  - intros gw i s1 s2 r1 (wB & gw' & Hs & Hse & HmB & Hm & Hf) Hr1.
+    edestruct @fsim_match_final_states as (r2 & gw1 & Hr2 & ACCO1 & ACCI1 & Hr); eauto.
+    exploit Hf; eauto. intros (gw2 &  ACCO2 & Hr2'). exists r2.
+    exists gw2. intuition auto.
+  - (*the most tricky part*)
+    intros gw2 i s1 s2 qA1 (wB & gw1 & Hs & Hse & HmB & Hm & Hf) HqA1.
+    edestruct @fsim_match_external as (wA & qA2 & Hacc1 & HqA2 & HqA & HseA & ?); eauto.
+    edestruct OUTGO as (wA' & Hm' & HseA' & HqA' & Hr); eauto.
+    exists wA', qA2. intuition auto.
+    exploit Hr; eauto. intros (wp1' & ACCO1 & MR1 & Hm'').
+    edestruct H as (i' & s2' & Hs2' & Hs'); eauto.
+    exists i', s2'. split; auto. exists wB. exists wp1'.
+    intuition auto.
+  - intros s1 t s1' Hs1' gw2 i s2 (wB & gw1 & Hs & Hse & Hr').
+   edestruct @fsim_simulation as (i' & s2' & Hs2' & Hs'); eauto.
+    exists i', s2'. split; auto.
+    econstructor; eauto.
+Qed.
+
+
+
+
+
+
